Regex/Data/String/Lemmas.lean
@@ -2,27 +2,24 @@ import Batteries.Data.String
 
 namespace String
 
-theorem valid_prev {p : Pos} (h : p.Valid s) : (prev s p).Valid s := by
-  match s, p, h with
-  | ⟨_⟩, ⟨_⟩, ⟨[], cs, rfl, rfl⟩ => simp_all
-  | ⟨_⟩, ⟨_⟩, ⟨cs, cs', rfl, rfl⟩ =>
+theorem valid_prev {p : Pos.Raw} (h : p.Valid s) : (Pos.Raw.prev s p).Valid s := by
+  match hm : s, p, h with
+  | _, ⟨_⟩, ⟨[], cs, _⟩ => simp_all
+  | _, ⟨_⟩, ⟨cs, cs', _⟩ =>
     match cs, cs.eq_nil_or_concat with
     | _, .inl rfl => simp_all
-    | _, .inr ⟨cs'', c, rfl⟩ =>
-      simp [String.Pos.Valid]
+    | cs, .inr ⟨cs'', c, h⟩ =>
       have := prev_of_valid cs'' c cs'
-      simp_all
-      exact ⟨cs'', And.intro ⟨c:: cs', rfl⟩ rfl⟩
+      exact Pos.Raw.Valid.intro ⟨cs'', ⟨c :: cs', by and_intros <;> simp_all⟩⟩
 
-theorem Pos.lt_def {a b : String.Pos} : a < b  ↔ a.byteIdx < b.byteIdx := Iff.rfl
+theorem Pos.lt_def {a b : String.Pos.Raw} : a < b  ↔ a.byteIdx < b.byteIdx := Iff.rfl
 
-theorem Pos.sub_lt_sub_left {k m n : String.Pos} (h1 : k < m) (h2 : k < n)
-    : m - n < m - k := by
+theorem Pos.sub_lt_sub_left {k m n : String.Pos.Raw} (h1 : k < m) (h2 : k < n)
+    : m.byteIdx - n.byteIdx < m.byteIdx - k.byteIdx := by
   have : m.byteIdx - n.byteIdx < m.byteIdx - k.byteIdx := Nat.sub_lt_sub_left h1 h2
   exact (String.Pos.lt_def.mpr this)
 
-theorem Pos.sizeof_lt_of_lt {a b : String.Pos} (h : a < b) : sizeOf a < sizeOf b := by
-  have sizeOf_string_pos {s : String.Pos} : sizeOf (s) = 1 + sizeOf s.byteIdx := rfl
-  simp at h
+theorem Pos.sizeof_lt_of_lt {a b : String.Pos.Raw} (h : a < b) : sizeOf a < sizeOf b := by
+  have sizeOf_string_pos {s : String.Pos.Raw} : sizeOf (s) = 1 + sizeOf s.byteIdx := rfl
   rw [sizeOf_string_pos, sizeOf_string_pos, sizeOf_nat, sizeOf_nat]
-  omega
+  exact Nat.add_lt_add_left h 1
